Moved to global array and removed admits

proof/correctness/NTT_Fq.ec
@@ -1,4 +1,4 @@
-require import AllCore IntDiv Array256.
+require import AllCore IntDiv Array256 Array128.
 require (****) ZModP.
 
 theory NTT_Fq.
@@ -6,19 +6,20 @@ theory NTT_Fq.
 clone import ZModP.
 
 module NTT = {
- proc ntt(r : zmod Array256.t,  zetas : zmod Array256.t) : zmod Array256.t = {
-   var len, start, j, k;
+ proc ntt(r : zmod Array256.t,  zetas : zmod Array128.t) : zmod Array256.t = {
+   var len, start, j, zetasctr;
    var  t, zeta_;
 
-   k <- 1;
+   zetasctr <- 0;
    len <- 128;
    while (2 <= len) {
     start <- 0;
     while(start < 256) {
-       zeta_ <- zetas.[k]; k <- k + 1;
+       zetasctr <- zetasctr + 1;
+       zeta_ <- zetas.[zetasctr]; 
        j <- start;
        while (j < start + len) {
-         t           <- zeta_ * r.[j + len];
+         t <- zeta_ * r.[j + len];
          r.[j + len] <- r.[j] + (-t);
          r.[j]       <- r.[j] + t;
          j <- j + 1;
@@ -30,16 +31,17 @@ module NTT = {
    return r;
  }
 
- proc invntt(r : zmod Array256.t, zetas_inv : zmod Array256.t) : zmod Array256.t = {
-   var len, start, j, k;
+ proc invntt(r : zmod Array256.t, zetas_inv : zmod Array128.t) : zmod Array256.t = {
+   var len, start, j, zetasctr;
    var  t, zeta_;
 
-   k <- 0;
+   zetasctr <- 0;
    len <- 2;
    while (len <= 128) {
     start <- 0;
     while(start < 256) {
-       zeta_ <- zetas_inv.[k]; k <- k + 1;
+       zeta_ <- zetas_inv.[zetasctr]; 
+       zetasctr <- zetasctr + 1;
        j <- start;
        while (j < start + len) {
         t <- r.[j];
