proof/correctness/KyberPoly.ec
@@ -1,0 +1,1188 @@
+require import List Int IntExtra IntDiv CoreMap IntDiv.
+from Jasmin require  import JModel JMemory.
+require import W16extra Array256 Array128.
+require import Fq.
+require import NTT_Fq.
+
+(* TODO: use easycrypt's native log to base *)
+op log2(n : int) : int.
+
+axiom log2E n l : 0 <= l => n = 2^l => log2 n = l.
+axiom log2pos n : 1 <= n => 0 <= log2 n.
+
+lemma logs :
+   log2 128 = 7 /\
+   log2 64  = 6 /\
+   log2 32  = 5 /\
+   log2 16  = 4 /\
+   log2 8   = 3 /\
+   log2 4   = 2 /\
+   log2 2   = 1 /\
+   log2 1   = 0
+  by smt(pow0 pow2_1 pow2_2 pow2_3 pow2_4 pow2_5 pow2_6 pow2_7  log2E log2pos).
+
+lemma logdiv2 n l :
+  1 < n =>
+  n = 2^l =>
+  log2 (n %/2) = log2 n - 1 by smt(@IntExtra log2E). 
+(**************)
+
+
+theory KyberPoly.
+
+import Fq.
+import ZModP.
+
+clone import NTT_Fq with
+   op ZModP.p <- Fq.q,
+   type ZModP.zmod <- zmod,
+   op ZModP.zero  <- Fq.ZModP.zero,
+   op ZModP.one   <- Fq.ZModP.one  ,
+   op ZModP.( + )  <- Fq.ZModP.( + ),
+   op ZModP.([-])  <- Fq.ZModP.([-]),
+   op ZModP.( * )  <- Fq.ZModP.( * ),
+   op ZModP.inv   <- Fq.ZModP.inv  ,
+   op ZModP.inzmod <- inzmod,
+   op ZModP.asint <- asint. (* .. *)
+
+import SignedReductions.
+
+op lift_array256 (p : W16.t Array256.t) =
+  Array256.map (fun x => inzmod (W16.to_sint x)) p.
+
+op lift_array128 (p : W16.t Array128.t) =
+  Array128.map (fun x => inzmod (W16.to_sint x)) p.
+
+op array_mont (p : zmod Array128.t) =
+  Array128.map (fun x => x *  (inzmod R)) p.
+
+op load_array_from_mem(mem : global_mem_t, ptr : W64.t) : W16.t Array256.t.
+
+axiom load_array_from_memE mem ptr i :
+   0 <= i < 256 =>
+     loadW16 mem (W64.to_uint ptr + 2* i) = (load_array_from_mem mem ptr).[i].
+
+op signed_bound_cxq(coefs : W16.t Array256.t, l u c : int) : bool =
+   forall k, l <= k < u => b16 coefs.[k] (c*Fq.q).
+
+op minimum_residues(zetas : W16.t Array128.t) : bool =
+   forall k, 0 <= k < 128 => bpos16  zetas.[k] Fq.q.
+
+require import Jasmin_poly.
+print M.
+
+lemma poly_add_corr _a _b ab bb :
+    0 <= ab <= 4 => 0 <= bb <= 4 =>  
+      hoare[ M.poly_add :
+           _a = lift_array256 ap /\
+           _b = lift_array256 bp /\
+           signed_bound_cxq ap 0 256 ab /\
+           signed_bound_cxq bp 0 256 bb 
+           ==>
+           signed_bound_cxq res 0 256 (ab + bb) /\ 
+           forall k, 0 <= k < 256 =>
+              inzmod (to_sint res.[k]) = _a.[k] + _b.[k]]. 
+move => *.
+proc. 
+while (
+           0 <= i <= 256 /\
+           _a = lift_array256 ap /\
+           _b = lift_array256 bp /\
+           signed_bound_cxq ap 0 256 ab /\
+           signed_bound_cxq bp 0 256 bb /\
+           signed_bound_cxq rp 0 i (ab + bb) /\ 
+           forall k, 0 <= k < i =>
+              inzmod (to_sint rp.[k]) = _a.[k] + _b.[k]
+); last by auto => />; smt(@Array256 @Fq). 
+
+wp; skip.
+move => &hr [#] *.
+split; first by smt().
+split; first by smt().
+split; first by smt().
+split; first by smt().
+split; first by smt().
+
+split; last first. 
+move => *.
+
+case (k < i{hr}); first by move => *; smt(@Array256). 
+
+move => *; rewrite (_: k =i{hr}) => />; first by smt().
+rewrite set_eqiE; first 2 by smt().
+
+move : (add_corr ap{hr}.[i{hr}] bp{hr}.[i{hr}] _a.[i{hr}] _b.[i{hr}] 14 14 _ _ _ _ _ _) => />; first 2 by smt(@Array256 @Fq). 
+move : H5; rewrite /signed_bound_cxq =>  *.
+move : (H5 k _); by smt(@Fq b16E).
+move : H6; rewrite /signed_bound_cxq =>  *.
+move : (H6 k _);  by smt(@Fq).
+
+rewrite /signed_bound_cxq.
+move => *.
+case (k < i{hr}); first by move => *; move : H7; rewrite /signed_bound_cxq;smt(@Array256). 
+
+move => *; rewrite (_: k =i{hr}) => />; first by smt().
+
+move : H5; rewrite /signed_bound_cxq =>  *.
+move : (H5 i{hr} _); first by smt().
+move : H6; rewrite /signed_bound_cxq =>  *.
+move : (H6 i{hr} _); first  by smt().
+move => *.
+rewrite /rp0.
+rewrite set_eqiE; first 2 by smt().
+rewrite !to_sintD_small; smt(@W16 @Fq b16E).
+qed.
+
+lemma poly_reduce_corr_h (_a : zmod Array256.t):
+      hoare[ M.poly_reduce :
+          _a = lift_array256 rp ==> 
+          _a = lift_array256 res /\
+          forall k, 0 <= k < 256 => bpos16  res.[k] (2*Fq.q)].
+proof.
+proc.
+exists *rp; elim* => _rp.
+conseq (_:
+  _rp = rp /\
+ (forall i, 0<= i < 256 =>
+              inzmod (to_sint rp.[i]) = _a.[i]) ==> 
+           forall i, 0<= i < 256 =>
+              to_sint rp.[i] = BREDC (to_sint _rp.[i]) 26
+). 
+move => &hr.
+rewrite /lift_array256 => /> *.
+rewrite mapiE => />.
+move => &hr.
+rewrite /lift_array256 => /> *.
+split.
+apply Array256.ext_eq => /> *.
+rewrite !mapiE => />.
+move : (H x _) => />.
+move : (BREDCp_corr (to_sint rp{hr}.[x]) 26 _ _ _ _ _);  by smt(@Fq @W16 @ZModP).
+move => *.
+move : (H k _) => />.
+move : (BREDCp_corr (to_sint rp{hr}.[k]) 26 _ _ _ _ _);  by smt(@Fq @W16).
+
+while (0 <= to_uint j <= 256 /\ 
+       (forall k, 0 <= k < to_uint j => to_sint rp.[k] = (BREDC (to_sint _rp.[k]) 26)) /\
+       (forall k, to_uint j <= k < 256 => to_sint rp.[k] =  (to_sint _rp.[k]))); last first.
+auto => />. 
+move => &ht H.
+split; first by smt().
+move => ??; move : H; rewrite ultE of_uintK => />; smt(@W16 @W64).
+move => *;wp; sp; ecall (barrett_reduce_corr_h (to_sint _rp.[to_uint j])); 
+ auto => />;smt(@W64 @Array256).
+qed.
+
+lemma poly_reduce_ll:
+  islossless M.poly_reduce
+ by proc;while (0 <= to_uint j <= 256) (256 - to_uint j); 
+   move=>*;inline *; auto => />;smt(@W64).
+
+lemma poly_reduce_corr (_a : zmod Array256.t):
+      phoare[ M.poly_reduce :
+          _a = lift_array256 rp ==> 
+          _a = lift_array256 res /\
+          forall k, 0 <= k < 256 => bpos16  res.[k] (2*Fq.q)] = 1%r.
+proof. by conseq poly_reduce_ll (poly_reduce_corr_h _a). qed.
+
+
+(*******DIRECT *******)
+lemma of_listW (p : W16.t -> bool) (xs : W16.t list) :
+      List.all p xs
+   => 128 <= size xs
+   => forall (i : int), 0 <= i < 128 => p ((Array128.of_list witness xs).[i]).
+proof.
+move=> pxs ge128_sz_xs i rg_i; rewrite get_of_list //. smt.
+qed.
+
+lemma zeta_bound :
+   minimum_residues jzetas.
+proof.
+rewrite /minimum_residues.
+apply/(allP jzetas (fun x => bpos16 x q)).
+auto => />.
+progress; by smt(@W16 @Fq).
+qed. 
+
+equiv ntt_correct &m :
+  NTT_Fq.NTT.ntt ~ M.poly_ntt : 
+        r{1} = lift_array256 rp{2} /\ 
+        array_mont zetas{1} = 
+           lift_array128  jzetas{2} /\
+        signed_bound_cxq rp{2} 0 256 2
+          ==> 
+            res{1} = lift_array256 res{2} /\
+            forall k, 0<=k<256 => bpos16 res{2}.[k] (2*Fq.q).
+proc.
+(* Dealing with final barret reduction *)
+seq 3 5 :  (r{1} = lift_array256 rp{2}); last first.
+ecall{2} (poly_reduce_corr (lift_array256 rp{2})).
+skip; move => &1 &2 [#] ?? [#] ??.
+split; first by smt (@Array256).
+by apply H1.
+
+(***********************************)
+
+seq 0 1: #pre; first by auto => />. 
+sp.
+
+(* Outer loop *)
+while (
+   zetasp{2} = jzetas /\
+   r{1} = lift_array256 rp{2} /\
+   array_mont zetas{1} = lift_array128 jzetas /\
+   len{1} = to_uint len{2} /\
+   zetasctr{1} = to_uint zetasctr{2}/\
+   (exists l, 0 <= l <= 7 /\ len{1} = 2^l) /\
+   0 <= zetasctr{1} <= 127 /\
+   2*(zetasctr{1}+1)*len{1} = 256 /\
+   signed_bound_cxq rp{2} 0 256 (9 - log2 len{1})); last 
+    by auto => />; move => *; split; [exists 7 => />; smt()| by smt(logs log2E)].
+wp; exists* zetasctr{1}; elim* => zetasctr1 l.
+
+(* Middle loop *)
+while (#{/~zetasctr1=zetasctr{1}}
+        {~2*(zetasctr{1}+1)*len{1} = 256}
+        {~signed_bound_cxq rp{2} 0 256 (9 - log2 len{1})}pre /\ 
+       2*(zetasctr1+1)*len{1}= 256 /\
+       start{1} = to_uint start{2} /\
+       0 <= start{1} <= 256 /\
+       start{1} = 2*(zetasctr{1} - zetasctr1)*len{1} /\
+       2* (zetasctr{1} - zetasctr1 ) * to_uint len{2} <= 256 /\
+       (* Nasty carry inv *)
+       signed_bound_cxq  rp{2} 0 256 (9 - log2 len{1} + 1) /\
+       signed_bound_cxq  rp{2} start{1} 256 (9 - log2 len{1})
+       ); last first.
+auto => />; move => &1 &2 zmont ????? cinv cbnd ??.
+split; first by  move : cbnd; rewrite /signed_bound_cxq => />; smt(@Fq).
+move => *;rewrite uleE !shr_div => />.
+split; last by  
+   rewrite (logdiv2 (to_uint len{2}) (log2 (to_uint len{2}))); 
+    [ smt(@W64) | smt(log2E) | smt(@W64) ]. 
+ by  exists (l-1); smt(@IntExtra).
+
+wp.
+
+(* Inner loop *)
+while (#{/~start{1} = 2*(zetasctr{1} - zetasctr1) * len{1}}
+        {~signed_bound_cxq  rp{2} start{1} 256 (9 - log2 len{1})} pre /\
+       zeta_{1}  *  (inzmod R) = inzmod (to_sint zeta_0{2}) /\  
+       0 <= to_sint zeta_0{2} < Fq.q /\
+       start{1} = 2*(zetasctr{1} -1 - zetasctr1) * len{1} /\
+       W64.to_uint cmp{2} = start{1} + len{1} /\ 
+       j{1} = to_uint j{2} /\
+       start{1} <= j{1} <= start{1} + len{1} /\
+       (
+       signed_bound_cxq  rp{2} (j{1}) (start{1} + len{1}) (9 - log2 len{1}) /\
+       signed_bound_cxq  rp{2} (j{1} + len{1}) 256 (9 - log2 len{1})
+       )
+       );last first. 
+auto => />. 
+move => &1 &2 ?? ? lenpow2 ??? ?? ???? cbdloose cbdtight ?? => />.
+
+split.
+
+(* Initialization *) 
+split; last by rewrite ultE to_uintD_small; by smt(@W64).
+split; first by rewrite !to_uintD_small of_uintK => />; smt(@IntExtra @W64).
+split. 
+rewrite to_uintD_small  => />; first by smt(@W64). 
+move : H; rewrite /array_mont /lift_array128 => *.
+have HH : (forall x, 0 <= x < 128 =>
+  (map (transpose Fq.ZModP.( * ) (inzmod R)) zetas{1}).[x] = (map (fun (x0 : W16.t) => inzmod (to_sint x0)) jzetas).[x]). 
+by rewrite H. 
+have ? : (to_uint zetasctr{2}  < 127); first by smt(@W64).
+move : (HH (to_uint zetasctr{2} + 1)_); first by smt().
+rewrite mapiE; first   by smt(@W64). 
+rewrite mapiE; first   by smt(@W64 @ZModP).
+split.
+have ? : (to_uint zetasctr{2}  < 127); first by smt(@W64).
+move : zeta_bound; rewrite /minimum_residues => /> AA; move : (AA (to_uint zetasctr{2} + 1) _); first by smt(@W64).
+rewrite !to_uintD_small; first 2 by smt(@W32).
+move => *.
+split;  first  by smt().
+split; first  by smt().
+split; first  by smt().
+move : cbdtight; rewrite /signed_bound_cxq => *.
+have ? : (to_uint start{2} + to_uint len{2} <= 256).
+rewrite -H6 H9; first by smt(@W64).
+split; move => *; move : (H15 k _); by smt().
+
+
+(* Termination *)
+move => *.
+split.
+rewrite (_:to_uint j_R = to_uint start{2} + to_uint len{2}); first by smt().
+split; [ by rewrite !to_uintD_small => />;  by smt(@W64) | by smt(@W64) ].
+by rewrite ultE /of_uingK to_uintD_small; smt(@W64).
+
+(* Preservation *)
+wp; sp. 
+ecall {2} (fqmul_corr (to_sint t{2}) (to_sint zeta_0{2})).
+skip => />.
+move => &1 &2 [#] mont ?? ?? ?? ??  ??? bloose ?? zetaval ?? -> cmp ?? btightsmall btightlarge ??? resval.
+
+move : btightlarge; rewrite /signed_bound_cxq => /> btightlarge. 
+ move : (btightlarge (to_uint (j{2} + len{2})) _);
+ rewrite to_uintD_small; first 3 by smt(@W16).  
+move : btightsmall; rewrite /signed_bound_cxq => /> btightsmall. 
+ move : (btightsmall (to_uint (j{2})) _); first by smt(@W16).
+move => jbound jlenboundl llenboundh.
+
+have bound1 : 2 <= to_uint len{2}; first by smt().
+have bound2 : (9 - log2 (to_uint len{2})) * Fq.q <= 8*Fq.q; first by smt(@W64 @Fq logs).
+have bound3 : -8*Fq.q <=  to_sint rp{2}.[to_uint j{2} + to_uint len{2}]<= 8*Fq.q; first by smt().
+have bound4 : -8*Fq.q <=  to_sint rp{2}.[to_uint j{2}]<= 8*Fq.q; first by smt().
+have bound5 : (-R %/ 2 * Fq.q < -8*Fq.q*Fq.q ); first by smt(@Fq).
+
+move :resval; rewrite to_uintD_small; first by smt(@W64). move => resval.
+
+move : (SREDCp_corr (to_sint rp{2}.[to_uint j{2} + to_uint len{2}] * to_sint zeta_0{2}) _ _); 
+  first 2 by have ? : (-R %/ 2 * Fq.q < -8*Fq.q*Fq.q ); smt(@Fq). 
+rewrite -!resval. move => sredc.
+
+split; last by smt(@W64).
+split; last first.
+split; first by smt(@W64).
+split; first by smt().
+
+(********* bounding carries *)
+(* tighter bound *)
+move => *.
+
+split; last first.
+(* part 1*)
+move => *.
+case (k <> to_uint j{2} /\ k <> to_uint j{2} + to_uint len{2}); first by 
+  move => *; rewrite !Array256.set_neqiE; smt(@W64). 
+  case (k = to_uint j{2}). 
+  move => *;rewrite !Array256.set_eqiE;  smt(@W64).
+  move => *; rewrite (_:k = to_uint j{2} + to_uint len{2}); first by smt().
+  rewrite Array256.set_neqiE; first 2 by smt(@W64). 
+  rewrite Array256.set_eqiE; by smt(@W64). 
+(* part 2 *)
+move => *.
+case (k <> to_uint j{2} /\ k <> to_uint j{2} + to_uint len{2}); first by 
+  move => *; rewrite !Array256.set_neqiE; smt(@W64). 
+  case (k = to_uint j{2}). 
+  move => *;rewrite !Array256.set_eqiE;  smt(@W64).
+  move => *; rewrite (_:k = to_uint j{2} + to_uint len{2}); first by smt().
+  rewrite Array256.set_neqiE; first 2 by smt(@W64). 
+  rewrite Array256.set_eqiE; by smt(@W64). 
+
+split; last first.
+(* looser bound *)
+move => *.
+rewrite (_: (10 - log2 (to_uint len{2})) * Fq.q = 
+            ( Fq.q) + ( (9 - log2 (to_uint len{2})) * Fq.q)); first by ring.
+case (k <> to_uint j{2} /\ k <> to_uint j{2} + to_uint len{2}). 
+  move => *; rewrite !Array256.set_neqiE; first 4 by smt(@W64). 
+       by move : bloose; rewrite /signed_bound_cxq; smt().
+    
+  case (k = to_uint j{2}). 
+  move => *;rewrite !Array256.set_eqiE; first 2 by smt(@W64).
+  rewrite to_sintD_small;  by smt(@Fq).
+  move => *;rewrite Array256.set_neqiE; first 2 by smt(@W64). 
+  rewrite Array256.set_eqiE; first 2 by smt(@W64). 
+  rewrite to_sintB_small;   by smt(@Fq).
+
+(*****************)
+(* One goal *)
+apply Array256.ext_eq.
+move => x xb => />.
+rewrite /lift_array256 !mapiE => />; first 2  by smt(@W64 @W16). 
+
+case (x <> to_uint j{2}). 
++ case (x <> to_uint j{2} + to_uint len{2}).
+   move => *.
+   rewrite Array256.set_neqiE; first 2 by smt(@W64).
+   rewrite Array256.set_neqiE; first 2 by smt(@W64).
+   rewrite Array256.set_neqiE; first 2 by smt(@W64).
+   rewrite Array256.set_neqiE; first 2 by smt(@W64).
+      rewrite mapiE; first by smt(). by auto => />. 
+   move => *.
+   rewrite Array256.set_neqiE; first 2 by smt(@W64).
+   rewrite Array256.set_eqiE; first 2 by smt(@W64). 
+   rewrite Array256.set_neqiE; first 2 by smt(@W64).
+   rewrite Array256.set_eqiE; first 2 by smt(@W64). 
+   rewrite to_sintB_small; first by smt(@Fq).
+
+   rewrite !inzmodB.
+   rewrite (_: inzmod (to_sint result) = 
+     inzmod (to_sint rp{2}.[to_uint j{2} + to_uint len{2}] * to_sint zeta_0{2} * 169)); first by smt( @ZModP).
+   rewrite !inzmodM -zetaval.
+   rewrite (_: inzmod (to_sint rp{2}.[to_uint j{2} + to_uint len{2}]) * (zeta_{1} * inzmod R) * inzmod 169 = 
+     inzmod (to_sint rp{2}.[to_uint j{2} + to_uint len{2}]) * ((zeta_{1} * inzmod R) * inzmod 169)); first by ring.
+   rewrite (_: (zeta_{1} * inzmod R) * inzmod 169 = zeta_{1}); first by smt(@ZModP RRinv).
+    by ring.
+
++ case (x <> to_uint j{2} + to_uint len{2}); last by smt(@Array256).
+   move => *; rewrite (_: x = to_uint j{2}); first by smt().
+   rewrite Array256.set_eqiE; first 2 by smt(@W64). 
+   rewrite Array256.set_neqiE; first 2 by smt(@W64).
+   rewrite Array256.set_eqiE; first 2 by smt(@W64). 
+   rewrite to_sintD_small; first by smt(@Fq).
+
+   rewrite !inzmodD.
+   rewrite (_: inzmod (to_sint result) = 
+      inzmod ((to_sint rp{2}.[to_uint j{2} + to_uint len{2}] * to_sint zeta_0{2} * 169))); first by smt(@ZModP).
+      rewrite !inzmodM -zetaval. 
+   rewrite (_: inzmod (to_sint rp{2}.[to_uint j{2} + to_uint len{2}]) * (zeta_{1} * inzmod R) * inzmod 169 = 
+     inzmod (to_sint rp{2}.[to_uint j{2} + to_uint len{2}]) * ((zeta_{1} * inzmod R) * inzmod 169)); first by ring.
+   rewrite (_: (zeta_{1} * inzmod R) * inzmod 169 = zeta_{1}); first by smt(@ZModP RRinv).
+   by ring; smt(@ZModP @Array256). 
+qed.
+
+(*******INVERSE *******)
+
+print M.
+
+lemma zetainv_bound :
+   minimum_residues jzetas_inv.
+proof.
+rewrite /minimum_residues.
+apply/(allP jzetas_inv (fun x => bpos16 x q)).
+auto => />.
+progress; by smt(@W16 @Fq).
+qed. 
+
+equiv invntt_correct &m :
+  NTT_Fq.NTT.invntt ~ M.poly_invntt : 
+        r{1} = lift_array256 rp{2} /\ 
+        array_mont zetas_inv{1} = 
+           lift_array128  jzetas_inv{2} /\
+        signed_bound_cxq rp{2} 0 256 2
+          ==> 
+            res{1} = lift_array256 res{2} /\
+            forall k, 0<=k<256 => b16 res{2}.[k] (Fq.q+1).
+proc.
+(* Dealing with final loop *)
+seq 3 5 :  (r{1} = lift_array256 rp{2} /\
+         zetasp{2} = jzetas_inv{2} /\
+        array_mont zetas_inv{1} = 
+           lift_array128  jzetas_inv{2} /\
+        signed_bound_cxq rp{2} 0 256 4
+); last first.
+while (j{1} = to_uint j{2} /\
+       0 <= j{1} <= 256 /\
+       r{1} = lift_array256 rp{2} /\
+       zetas_inv.[127]{1} * inzmod R  = inzmod (to_sint jzetas_inv{2}.[127]) /\
+       zeta_0{2} = jzetas_inv{2}.[127] /\
+       signed_bound_cxq rp{2} 0 256 4 /\
+       (forall k, 0 <= k < j{1} =>
+           b16 rp{2}.[k] (Fq.q + 1))
+); last first. 
+  wp;skip; move => &1 &2 [#] -> zp zvals zbnd??.
+  split; last by smt(@W64 b16E @Array256).
+  split; last by rewrite ultE;  smt(@W64).
+  split; first by smt(@W64).
+  split; first by smt().
+  split; first by smt().
+  split.
+  move : zvals; rewrite /lift_array128 /array_mont => H.
+have HH : (forall x, 0 <= x < 128 =>
+  (map (transpose Fq.ZModP.( * ) (inzmod R)) zetas_inv{1}).[x] = (map (fun (x0 : W16.t) => inzmod (to_sint x0)) jzetas_inv).[x]). 
+by rewrite H. 
+move : (HH (127)_); first by smt().
+rewrite mapiE => />.  
+split; first by  rewrite /zeta_0_R zp.
+split; last  by smt().
+move : zbnd; rewrite /signed_bound_cxq; smt(@Array256).
+
+sp;wp;ecall{2} (fqmul_corr (to_sint t{2}) (to_sint jzetas_inv.[127])).
+
+skip => />; move => &1 &2 ?? zetaval  cbound tightbound ???resval.
+
+move : cbound; rewrite /signed_bound_cxq => /> cbound. 
+move : (cbound (to_uint j{2}) _) => />.
+move => jboundl jboundh.
+
+have bound4 : -4*Fq.q <=  to_sint rp{2}.[to_uint j{2}]<= 4*Fq.q; first by smt().
+have bound5 : (-R %/ 2 * Fq.q < -4*Fq.q*Fq.q ); first by smt(@Fq).
+
+move :resval; rewrite to_uintD_small; first by smt(@W64). move => resval.
+
+move : (SREDCp_corr (to_sint rp{2}.[to_uint j{2}] * to_sint ((W16.of_int 1441))) _ _).
+ smt(@Fq).  
+have ? : (-R %/ 2 * Fq.q < -4*Fq.q* to_sint ((of_int 1441))%W16 ); first   by smt(@Fq @W16).
+simplify => />. move : (cbound (to_uint j{2}) _); first  by smt(@Fq).
+move => * />. 
+split; smt(@W16 @Fq).
+
+move => *.
+split. 
+split; first by smt(@W64).
+split; first by smt(@W64).
+split; last first.
+split. 
+
+move => *.
+case (k = to_uint j{2}).
+   move => ->; rewrite !Array256.set_eqiE; smt(@W64). 
+   by move => *;rewrite !Array256.set_neqiE; smt(@W64). 
+move => *.
+case (k = to_uint j{2}).
+   by move => ->; rewrite !Array256.set_eqiE; smt(@W64). 
+   by move => *;rewrite !Array256.set_neqiE; smt(@W64). 
+
+apply Array256.ext_eq.
+move => x xbnd.
+   rewrite /lift_array256 !mapiE; first 2 by smt().
+   case (x = to_uint j{2}).
+   move => ->; rewrite !Array256.set_eqiE; first 4 by smt(@W64). 
+   rewrite (_: zetas_inv{1}.[127] = inzmod (to_sint ((W16.of_int 1441)) * 169)).
+       rewrite inzmodM -zetaval.
+       rewrite (_: zetas_inv{1}.[127] * inzmod R * inzmod 169 =
+                    zetas_inv{1}.[127] * (inzmod R * inzmod 169)); first by ring.
+   smt(@ZModP RRinv). smt(@ZModP).
+   move => *; rewrite !Array256.set_neqiE; by smt(@Array256). 
+
+by rewrite ultE; smt(@W64).
+
+(***********************************)
+
+sp.
+(* Outer loop *)
+while (
+   zetasp{2} = jzetas_inv /\
+   r{1} = lift_array256 rp{2} /\
+   array_mont zetas_inv{1} = lift_array128 jzetas_inv /\
+   len{1} = to_uint len{2} /\
+   (exists l, 1 <= l <= 8 /\ len{1} = 2^l) /\
+   0 <= zetasctr{1} <= 128 /\
+   zetasctr{1} = to_uint zetasctr{2} /\
+   zetasctr{1} * len{1} = 128 * (len{1} - 2) /\
+   signed_bound_cxq rp{2} 0 256 4); last first.
+auto => />. move => &1 &2 ??.
+split; first by exists (1);  smt(logs).
+move : H0; rewrite /signed_bound_cxq;smt(@Array256 @Fq).
+
+wp; exists* zetasctr{1}; elim* => zetasctr1 l.
+
+(* Middle loop *)
+while (#{/~zetasctr1=zetasctr{1}}
+        {~zetasctr{1} * len{1} = 128 * (len{1} - 2)}pre /\ 
+       zetasctr1 * len{1} = 128 * (len{1} - 2) /\
+       start{1} = to_uint start{2} /\
+       0 <= start{1} <= 256 /\
+       start{1} = 2*(zetasctr{1} - zetasctr1)*len{1} /\
+       2* (zetasctr{1} - zetasctr1) * to_uint len{2} <= 256 /\
+       (* Nasty carry inv *)
+       signed_bound_cxq  rp{2} 0 256 4); last first.
+auto => />; move => *.
+rewrite /(W64.(`<<`)) !uleE !of_uintK !to_uint_shl=> />.
+split; last by smt(@W64).
+split; first by rewrite modz_small; smt(@IntExtra).
+split; last by smt(). 
+exists (l+1); smt(@IntExtra log2E logs).
+
+wp.
+
+(* Inner loop *)
+while (#{/~start{1} = 2*(zetasctr{1} - zetasctr1) * len{1}} pre /\
+       zeta_{1}  *  (inzmod R) = inzmod (to_sint zeta_0{2}) /\  
+       0 <= to_sint zeta_0{2} < Fq.q /\
+       start{1} = 2*((zetasctr{1}-1) - zetasctr1) * len{1} /\
+       W64.to_uint cmp{2} = start{1} + len{1} /\ 
+       j{1} = to_uint j{2} /\
+       start{1} <= j{1} <= start{1} + len{1}); last first.
+auto => />. 
+move => &1 &2 zetasd ?? lenpow2 ?? cbd ????????? => />.
+
+split.
+
+(* Initialization *) 
+split; last by rewrite ultE to_uintD_small; by smt(@W64).
+split.
+split.
+by smt(@W64).
+split; first by smt().
+split; last by smt( logs log2E).
+rewrite to_uintD_small; smt(@W64).
+
+split. 
+move : zetasd; rewrite /array_mont /lift_array128.
+move => zz.
+have ? :(forall k, 0 <= k < 128 => 
+  (map (transpose Fq.ZModP.( * ) (inzmod R)) zetas_inv{1}).[k] = (map (fun (x : W16.t) => inzmod (to_sint x)) jzetas_inv).[k]).
+by rewrite zz.
+move : (H12 (to_uint zetasctr{2})_); first by smt().
+rewrite mapiE; first by smt().
+rewrite mapiE; first by smt().
+simplify => />.
+
+split; last by rewrite to_uintD_small;  smt(@W64).
+
+move : zetainv_bound; rewrite /minimum_residues => zbnd; 
+  move : (zbnd (to_uint zetasctr{2}) _);  smt(@W64).
+
+(* Termination *)
+move => *.
+split.
+rewrite (_:to_uint j_R = to_uint start{2} + to_uint len{2}); first by smt().
+split; [ by rewrite !to_uintD_small => />;  by smt(@W64) | by smt(@W64) ].
+by rewrite ultE /of_uingK to_uintD_small; smt(@W64).
+
+(* Preservation *)
+
+(*  Dealing with barrett reduction *)
+wp; sp; exists* m{2}; elim* => m2.
+seq 0 1 : (#{/~m2=m{2}}{~ m{2} = s{2} + t{2}}pre /\ 
+          inzmod (to_sint m{2}) = inzmod(to_sint (s{2} + t{2})) /\ 
+          bpos16 m{2} (2*Fq.q)).
+ecall {2}  (barrett_reduce_corr (to_sint m2)) => />; first by  smt().
+auto => />.
+move => &1 &2 [#] ?? ?? ??   cbnd ?????? ?? zetaval ?? -> ?????? resval.
+
+move : cbnd; rewrite /signed_bound_cxq => /> cbnd. 
+ move : (cbnd (to_uint (j{2} + len{2})) _).
+ rewrite to_uintD_small;   by smt(@W16 @W64). move => jlenbound.
+ move : (cbnd (to_uint j{2}) _); first by by smt(@W64). move => jbound.
+
+move : resval.
+rewrite !to_uintD_small; first by smt(@W64).
+move  :  (BREDCp_corr (to_sint (rp{2}.[to_uint j{2} + to_uint len{2}] + rp{2}.[to_uint j{2}])) 26 _ _ _ _ _) => />; first 3 by smt(@Fq).
+move : jlenbound jbound cbnd; rewrite qE /R !to_uintD_small => /> *; first by smt(@W16). 
+rewrite to_sintD_small; smt(@W16).
+
+by move => ??? resval; smt(@ZModP).
+
+(* Dealing with the multiplication *)
+sp.
+
+ecall {2} (fqmul_corr (to_sint t{2}) (to_sint zeta_0{2})).
+skip => />.
+move => &1 &2 rP_R [#] ?   ????? cbnd ??? ?? ? ?? zetaval ?? -> cmp ???? ???? resval.
+
+move : cbnd; rewrite /signed_bound_cxq => /> cbnd. 
+ move : (cbnd (to_uint (j{2} + len{2})) _); first by smt(@W16 @W64).
+ rewrite !to_uintD_small;  first 2  by smt(@W16 @W64). move => /> jlenboundl jlenboundh.
+ move : (cbnd (to_uint j{2}) _); first by smt(@W64). move => /> jboundl jboundh.
+
+have bound1 : 2 <= to_uint len{2}; first by smt(@IntExtra).
+have bound2 : (-R %/ 2 < -4*Fq.q ); first by smt(@Fq).
+have bound3 : (-R %/ 2 * Fq.q < -4*Fq.q*Fq.q ); first by smt(@Fq).
+
+move : resval.
+rewrite !to_uintD_small; first by smt(@W64).
+move : (SREDCp_corr (to_sint (rP_R.[to_uint j{2}] - rP_R.[to_uint j{2} + to_uint len{2}]) * to_sint zeta_0{2}) _ _) => />; first  by smt(@Fq).
+ rewrite !to_sintD_small => />.  
+
+rewrite !to_sintN;  by smt(@Fq).
+rewrite !to_sintN;  by smt(@Fq).
+
+ move => resbl resbh rescong resval.
+
+split; last by smt(@W64).
+split; last smt(@W64).
+
+(********* bounding carries *)
+split; last first.
+split.
+(* part 1*)
+move => *.
+case (k <> to_uint j{2} /\ k <> to_uint j{2} + to_uint len{2}); first by 
+  move => *; rewrite !Array256.set_neqiE; smt(@W64). 
+  case (k = to_uint j{2}). 
+  move =>  ->;rewrite Array256.set_neqiE; first 2  by smt(@W64). 
+  rewrite Array256.set_eqiE;   by smt(@W64). 
+  move => *; rewrite (_:k = to_uint j{2} + to_uint len{2}); first by smt().
+  rewrite Array256.set_eqiE; first 2 by smt(@W64). 
+ rewrite resval; smt(@Fq).
+
+(* part 2 *)
+move => *.
+case (k <> to_uint j{2} /\ k <> to_uint j{2} + to_uint len{2}); first by 
+  move => *; rewrite !Array256.set_neqiE; smt(@W64). 
+  case (k = to_uint j{2}). 
+  move => *. rewrite Array256.set_neqiE; first 2 by smt(@W64).
+  move => *. rewrite Array256.set_eqiE; by smt(@W64).
+  move => *; rewrite (_:k = to_uint j{2} + to_uint len{2}); first by smt().
+  rewrite Array256.set_eqiE;  by smt(@W64). 
+
+(*****************)
+(* One goal *)
+apply Array256.ext_eq.
+move => x xb => />.
+rewrite /lift_array256 !mapiE => />; first 2  by smt(@W64 @W16). 
+
+case (x <> to_uint j{2} + to_uint len{2}). 
++ case (x <> to_uint j{2}); first by smt(@Array256).
+   move => *.
+   rewrite Array256.set_neqiE; first 2 by smt(@W64).
+   rewrite Array256.set_eqiE; first 2 by smt(@W64). 
+   rewrite Array256.set_neqiE; first 2 by smt(@W64).
+   rewrite Array256.set_eqiE; first 2 by smt(@W64). 
+   rewrite H19.
+   rewrite !to_sintD_small to_uintD_small; first  by smt(@Fq @W64).
+   simplify => />. smt(@Fq @W16).
+   simplify => />. smt(@Fq @W16).
+   by rewrite !inzmodD; ring.
+
++ case (x <> to_uint j{2}); last by smt(@Array256).
+   move => *; rewrite (_: x = to_uint j{2}  + to_uint len{2}); first by smt().
+   rewrite Array256.set_eqiE; first 2 by smt(@W64). 
+   rewrite Array256.set_eqiE; first 2 by smt(@W64).
+   rewrite Array256.set_neqiE; first 2 by smt(@W64). 
+   rewrite Array256.set_eqiE; first 2 by smt(@W64). 
+   rewrite mapiE; first by smt(@W64).
+   rewrite resval => />. 
+   rewrite (_: 
+     inzmod (SREDC (to_sint (rP_R.[to_uint j{2}] - rP_R.[to_uint j{2} + to_uint len{2}]) * to_sint zeta_0{2})) = 
+     inzmod ((to_sint (rP_R.[to_uint j{2}] - rP_R.[to_uint j{2} + to_uint len{2}]) * to_sint zeta_0{2} * 169))); first by smt(@ZModP).
+   rewrite (_: zeta_{1} = inzmod (to_sint zeta_0{2} * 169)).
+       rewrite inzmodM -zetaval.
+       rewrite (_: zeta_{1} * inzmod R * inzmod 169 =
+                    zeta_{1} * (inzmod R * inzmod 169)); first by ring.
+   smt(@ZModP RRinv). 
+   rewrite !to_sintD_small. rewrite to_sintN /R => />;  smt(@Fq @W16). 
+   rewrite !to_sintN; first  by smt(@Fq @W64).
+   by rewrite -inzmodB !inzmodM; ring.
+qed.
+
+(* COMPLEX MULTIPLICATION *)
+
+print M.
+
+op complex_mul (a :zmod * zmod, b : zmod * zmod, zzeta : zmod) =
+     (a.`2 * b.`2 * zzeta * (inzmod 169) + a.`1*b.`1  * (inzmod 169), 
+      a.`1 * b.`2  * (inzmod 169) + a.`2 * b.`1  * (inzmod 169)).
+
+op double_mul(a1 : zmod * zmod, b1 : zmod * zmod, 
+              a2 : zmod * zmod, b2 : zmod * zmod, zzeta : zmod) = 
+     (complex_mul a1 b1 zzeta, complex_mul a2 b2 (-zzeta)).
+
+op base_mul(ap bp : zmod Array256.t, zetas : zmod Array128.t, rs : zmod Array256.t, i : int) : bool = 
+   forall k, 0 <= k < i =>
+     ((rs.[4*k],rs.[4*k+1]),(rs.[4*k+2],rs.[4*k+3])) =
+         (double_mul (ap.[4*k],ap.[4*k+1]) (bp.[4*k],bp.[4*k+1])
+                    (ap.[4*k+2],ap.[4*k+3]) (bp.[4*k+2],bp.[4*k+3]) (zetas.[k+64])).
+
+print M.
+
+lemma poly_basemul_corr _ap _bp _zetas:
+      hoare[ M.poly_basemul :
+        array_mont _zetas = 
+           lift_array128 jzetas /\
+           _ap = lift_array256 ap /\
+           _bp = lift_array256 bp /\
+           signed_bound_cxq ap 0 256 2 /\
+           signed_bound_cxq bp 0 256 2 ==>
+             signed_bound_cxq res 0 256 4 /\
+             base_mul _ap _bp _zetas (lift_array256 res) 64].
+proof.
+move => *.
+proc.
+seq 2 : #pre; first by auto => />.
+sp.
+while (#{/~i=0}{~zetasctr = W64.of_int 64}pre /\
+    0<= i <= 64/\
+    to_uint zetasctr = i + 64 /\
+    signed_bound_cxq rp 0 (4*i) 4 /\
+    base_mul _ap _bp _zetas (lift_array256 rp) i); last first. 
+    auto => />.
+    move => *; split; first by smt(). 
+    move => *; have ? : i0 = 64; first by smt(). 
+    by move : H6 H7; rewrite H8 => />. 
+
+seq 2 : (#{/~to_uint zetasctr = i + 64}pre /\ inzmod (to_sint zeta_0) = 
+            _zetas.[i + 64] * inzmod R /\
+            to_uint zetasctr - 1 = i + 64 /\
+             bpos16 zeta_0 Fq.q).
+
+auto => />.
+move => &hr mnt abnd bbnd? ??? rbndrval ?.
+move :mnt; rewrite /minimum_residues /array_mont /lift_array128. 
+move => ?.
+split; first by rewrite H1; smt(@Array128).
+split; first by rewrite to_uintD_small H1; smt(@W64).
+move : zeta_bound; rewrite /minimum_residues =>/>.
+by rewrite qE to_sintE => />; smt(@W16).
+
+(* First complex multiplication *)
+
+seq  13 : (#pre /\
+           (inzmod (to_sint rp.[4*i]),inzmod (to_sint rp.[4*i+1])) = 
+             complex_mul (inzmod (to_sint ap.[4*i]),inzmod (to_sint ap.[4*i+1])) 
+                         (inzmod (to_sint bp.[4*i]),inzmod (to_sint bp.[4*i+1])) 
+                         (_zetas.[64+i]) /\
+             b16 rp.[4*i] (4*Fq.q) /\ b16 rp.[4*i+1] (4*Fq.q)).
+
+
+sp;wp.
+seq 4 : (#pre /\
+          inzmod (to_sint r0) = 
+           inzmod (to_sint ap.[4*i+1]) * inzmod (to_sint bp.[4*i+1]) * 
+           _zetas.[64+i] * (inzmod 169)  + 
+           inzmod (to_sint ap.[4*i]) * inzmod (to_sint bp.[4*i])  * (inzmod 169) /\
+           b16 r0 (4*Fq.q)
+        ).
+seq 1 : (#pre /\
+           inzmod (to_sint r0) = 
+           inzmod (to_sint ap.[4*i+1]) * inzmod (to_sint bp.[4*i+1])  * (inzmod 169) /\
+           b16 r0 (2*Fq.q)).
+ecall (fqmul_corr_h (to_sint a1) (to_sint b1)).
+auto => />. 
+move => &hr mont bas bbs ?? pbnd  ?????? ? rval.
+
+move : (SREDCp_corr (to_sint ap{hr}.[4 * i{hr} + 1] * to_sint bp{hr}.[4 * i{hr} + 1]) _ _) => />; first by smt(@Fq). 
+
+move : bas; rewrite /signed_bound_cxq => /> bas. 
+ move : (bas ( (4*i{hr} + 1)) _); first by smt().
+ move : (bas (4*i{hr}) _); first by smt(@W64). move => aibnd ai1bnd.
+
+move : bbs; rewrite /signed_bound_cxq => /> bbs. 
+ move : (bbs ( (4*i{hr} + 1)) _); first by smt().
+ move : (bbs (4*i{hr}) _); first by smt(@W64). move => bibnd bi1bnd.
+
+smt(@Fq @W16).
+by rewrite eq_inzmod -rval !inzmodM; smt(@Fq).
+
+seq 1 : (#{~inzmod (to_sint r0) = inzmod (to_sint ap.[4 * i + 1]) * inzmod (to_sint bp.[4 * i + 1]) * inzmod 169}pre /\
+           inzmod (to_sint r0) = 
+           inzmod (to_sint ap.[4*i+1]) * inzmod (to_sint bp.[4*i+1]) *
+               _zetas.[i+64] * (inzmod 169) /\
+           b16 r0 (2*Fq.q)).
+ecall (fqmul_corr_h (to_sint r0) (to_sint zeta_0)).
+auto => />. 
+move => &hr mont bas bbs ??pbndt  ??zetaval ??? r0val ???rval.
+
+move : (SREDCp_corr (to_sint r0{hr} * to_sint zeta_0{hr}) _ _) => />;
+  first 2 by smt(@Fq). 
+
+rewrite eq_inzmod -rval !inzmodM r0val. 
+
+move => ?? ->.
+
+split; first by  smt(@Fq).
+split; last by  smt(@Fq).
+
+rewrite zetaval.
+have ? : (inzmod (to_sint ap{hr}.[4 * i{hr} + 1]) * inzmod (to_sint bp{hr}.[4 * i{hr} + 1]) * inzmod 169 *
+(_zetas.[64 + i{hr}] * inzmod R) * inzmod 169 =
+inzmod (to_sint ap{hr}.[4 * i{hr} + 1]) * inzmod (to_sint bp{hr}.[4 * i{hr} + 1]) * inzmod 169 *
+_zetas.[64 + i{hr}] * (inzmod (R * 169))
+); first by  rewrite inzmodM; ring. by smt(@ZModP RRinv).
+
+wp.
+ecall (fqmul_corr_h (to_sint a0) (to_sint b0)).
+auto => />. 
+move => &hr mnt bas bbs ?? rbnd rv ? zval ????? r0val ?rval.
+
+move : bas; rewrite /signed_bound_cxq => /> bas. 
+ move : (bas ( (4*i{hr} + 1)) _); first by smt().
+ move : (bas (4*i{hr}) _); first by smt(@W64). move => aibnd ai1bnd.
+
+move : bbs; rewrite /signed_bound_cxq => /> bbs. 
+ move : (bbs ( (4*i{hr} + 1)) _); first by smt().
+ move : (bbs (4*i{hr}) _); first by smt(@W64). move => bibnd bi1bnd.
+
+move : (SREDCp_corr (to_sint ap{hr}.[4 * i{hr}] * to_sint bp{hr}.[4 * i{hr}]) _ _) => />;
+  first 2 by smt(@Fq). 
+
+rewrite eq_inzmod -rval !inzmodM. 
+move => ?? rrval.
+
+rewrite !to_sintD_small. smt(@Fq).
+split.
+rewrite  !inzmodD rrval => /#.
+by smt(@Fq).
+
+ecall (fqmul_corr_h (to_sint a1) (to_sint b0)).
+ecall (fqmul_corr_h (to_sint a0) (to_sint b1)).
+
+auto => />.
+
+move => &hr mnt bas bbs ?? rbnd rv ? zval ??? r0val ??? rval ?rvall. 
+
+move : bas; rewrite /signed_bound_cxq => /> bas. 
+ move : (bas ( (4*i{hr} + 1)) _); first by smt().
+ move : (bas (4*i{hr}) _); first by smt(@W64). move => aibnd ai1bnd.
+
+move : bbs; rewrite /signed_bound_cxq => /> bbs. 
+ move : (bbs ( (4*i{hr} + 1)) _); first by smt().
+ move : (bbs (4*i{hr}) _); first by smt(@W64). move => bibnd bi1bnd.
+
+split. split.
+
+move => k kl kh.
+case (k = 4 * i{hr}). smt(@Array256 @Fq). 
+case (k = 4 * i{hr}+1). smt(@Array256 @Fq). 
+
+move => *.
+rewrite Array256.set_neqiE; first 2 by smt(@W64). 
+rewrite Array256.set_neqiE; first 2 by smt(@W64). 
+
+move : rbnd; rewrite /signed_bound_cxq => rbnd. 
+move : (rbnd k). rewrite b16E.
+smt(@Fq).
+
+rewrite /base_mul.
+move => k kb.
+rewrite /lift_array256 !mapiE; first 12 by smt(). 
+
+rewrite !Array256.set_neqiE; first 16 by smt(@W64). 
+
+simplify => />.
+
+move : rv; rewrite /base_mul => rv.
+
+move : (rv k kb).
+rewrite /lift_array256 !mapiE; first 12 by smt(). 
+simplify => />.
+
+move : (SREDCp_corr (to_sint ap{hr}.[4 * i{hr}] * to_sint bp{hr}.[4 * i{hr} + 1]) _ _) => />;
+  first 2 by smt(@Fq). 
+
+rewrite eq_inzmod -rval !inzmodM. 
+move => ?? rrval.
+
+
+move : (SREDCp_corr (to_sint ap{hr}.[4 * i{hr} + 1] * to_sint bp{hr}.[4 * i{hr}]) _ _) => />;
+  first 2 by smt(@Fq). 
+
+rewrite eq_inzmod -rvall !inzmodM. 
+move => ?? rrvall.
+
+rewrite Array256.set_neqiE; first 2 by smt(@W64). 
+rewrite Array256.set_eqiE; first 2 by smt(@W64). 
+rewrite Array256.set_eqiE; first 2 by smt(@W64). 
+
+
+rewrite !to_sintD_small. smt(@Fq @W16).
+rewrite r0val inzmodD rrval rrvall.
+split. split; by ring.
+smt(@W16 @Fq).
+
+(* Second complex multiplication *)
+
+seq 1 : (#{/~inzmod (to_sint zeta_0) = _zetas.[i + 64] * inzmod R}
+          {~bpos16 zeta_0 Fq.q}pre /\
+          inzmod (to_sint zeta_0) = - _zetas.[i + 64] * inzmod R /\
+          -Fq.q < to_sint zeta_0 <= 0).
+auto => />. 
+move => *. split. rewrite to_sintN => />. 
+move : H9 H10. 
+rewrite to_sintE /smod qE => />; smt(@W16).
+smt(@ZModP). 
+rewrite to_sintN => />.  
+move : H9 H10; rewrite qE => />; smt(@W16). 
+move : H9 H10; rewrite qE => />; smt(@W16). 
+
+seq  13 : (#pre /\
+           (inzmod (to_sint rp.[4*i+2]),inzmod (to_sint rp.[4*i+3])) = 
+             complex_mul (inzmod (to_sint ap.[4*i+2]),inzmod (to_sint ap.[4*i+3])) 
+                         (inzmod (to_sint bp.[4*i+2]),inzmod (to_sint bp.[4*i+3])) 
+                         (-_zetas.[64+i]) /\
+             b16 rp.[4*i+2] (4*Fq.q) /\ b16 rp.[4*i+3] (4*Fq.q)).
+
+sp;wp.
+seq 4 : (#pre /\
+          inzmod (to_sint r0) = 
+           inzmod (to_sint ap.[4*i+3]) * inzmod (to_sint bp.[4*i+3]) * 
+           (-_zetas.[64+i]) * (inzmod 169)  + 
+           inzmod (to_sint ap.[4*i+2]) * inzmod (to_sint bp.[4*i+2])  * (inzmod 169) /\
+           b16 r0 (4*Fq.q)
+        ).
+seq 1 : (#pre /\
+           inzmod (to_sint r0) = 
+           inzmod (to_sint ap.[4*i+3]) * inzmod (to_sint bp.[4*i+3])  * (inzmod 169) /\
+           b16 r0 (2*Fq.q)).
+ecall (fqmul_corr_h (to_sint a1) (to_sint b1)).
+auto => />. 
+move => &hr mont bas bbs ?? rb rv ???????? zval zbl zbh ? rval.
+
+move : (SREDCp_corr (to_sint ap{hr}.[4 * i{hr} + 3] * to_sint bp{hr}.[4 * i{hr} + 3]) _ _) => />; first by smt(@Fq). 
+
+move : bas; rewrite /signed_bound_cxq => /> bas. 
+ move : (bas ( (4*i{hr} + 3)) _); first by smt().
+ move : (bas (4*i{hr}+2) _); first by smt(@W64). move => aibnd ai1bnd.
+
+move : bbs; rewrite /signed_bound_cxq => /> bbs. 
+ move : (bbs ( (4*i{hr} + 3)) _); first by smt().
+ move : (bbs (4*i{hr}+2) _); first by smt(@W64). move => bibnd bi1bnd.
+
+smt(@Fq @W16).
+by rewrite eq_inzmod -rval !inzmodM; smt(@Fq).
+
+seq 1 : (#{~inzmod (to_sint r0) = inzmod (to_sint ap.[4 * i + 3]) * inzmod (to_sint bp.[4 * i + 3]) * inzmod 169}pre /\
+           inzmod (to_sint r0) = 
+           inzmod (to_sint ap.[4*i+3]) * inzmod (to_sint bp.[4*i+3]) *
+               -_zetas.[i+64] * (inzmod 169) /\
+           b16 r0 (2*Fq.q)).
+ecall (fqmul_corr_h (to_sint r0) (to_sint zeta_0)).
+auto => />.
+move => &hr mont bas bbs ?? rb rv ???????? zval zbl zbh  r0val ???rval.
+
+move : (SREDCp_corr (to_sint r0{hr} * to_sint zeta_0{hr}) _ _) => />.
+  by smt(@Fq). 
+  by smt(@Fq). 
+
+rewrite eq_inzmod -rval !inzmodM r0val. 
+
+move => ?? ->.
+
+split; first by  smt(@Fq).
+split; last by  smt(@Fq).
+
+rewrite zval.
+have aux : (inzmod (to_sint ap{hr}.[4 * i{hr} + 3]) * inzmod (to_sint bp{hr}.[4 * i{hr} + 3]) * inzmod 169 *
+- _zetas.[64 + i{hr}] * inzmod R * inzmod 169 =
+(inzmod R * inzmod 169) * inzmod (to_sint ap{hr}.[4 * i{hr} + 3]) * inzmod (to_sint bp{hr}.[4 * i{hr} + 3]) *
+- _zetas.[64 + i{hr}]  * inzmod 169
+); first by ring. 
+move : aux.
+rewrite (_: (inzmod R * inzmod 169)= inzmod (R*169)); first by rewrite inzmodM.
+move : RRinv; rewrite eq_inzmod => ->.
+rewrite (_: inzmod 1 = Fq.ZModP.one); first by smt(@ZModP). 
+rewrite ZModP.ComRing.mul1r. 
+rewrite (_: i{hr} + 64 = 64+ i{hr}); first by ring.
+pose a := inzmod (to_sint ap{hr}.[4 * i{hr} + 3]).
+pose b := inzmod (to_sint bp{hr}.[4 * i{hr} + 3]).
+pose z := _zetas.[64 + i{hr}].
+pose c := inzmod 169.
+pose d := inzmod R.
+move => XX; rewrite -XX. 
+by ring.
+
+wp.
+ecall (fqmul_corr_h (to_sint a0) (to_sint b0)).
+auto => />. 
+move => &hr mont bas bbs ?? rb rv ???????? zval zbl zbh  r0val ???rval.
+
+move : bas; rewrite /signed_bound_cxq => /> bas. 
+ move : (bas ( (4*i{hr} + 3)) _); first by smt().
+ move : (bas (4*i{hr} + 2) _); first by smt(@W64). move => aibnd ai1bnd.
+
+move : bbs; rewrite /signed_bound_cxq => /> bbs. 
+ move : (bbs ( (4*i{hr} + 3)) _); first by smt().
+ move : (bbs (4*i{hr} + 2) _); first by smt(@W64). move => bibnd bi1bnd.
+
+move : (SREDCp_corr (to_sint ap{hr}.[4 * i{hr} + 2] * to_sint bp{hr}.[4 * i{hr} + 2]) _ _) => />;
+  first 2 by smt(@Fq). 
+
+rewrite eq_inzmod -rval !inzmodM. 
+move => ?? rrval.
+
+rewrite !to_sintD_small. smt(@Fq).
+split.
+rewrite  !inzmodD rrval H10.
+rewrite (_: i{hr} + 64 = 64+ i{hr});  by ring.
+smt(@Fq).
+
+ecall (fqmul_corr_h (to_sint a1) (to_sint b0)).
+ecall (fqmul_corr_h (to_sint a0) (to_sint b1)).
+
+auto => />.
+move => &hr mont bas bbs ?? rb rv ???????? zval zbl zbh  r0val ???rval ?rvall. 
+
+move : bas; rewrite /signed_bound_cxq => /> bas. 
+ move : (bas ( (4*i{hr} + 3)) _); first by smt().
+ move : (bas (4*i{hr}+2) _); first by smt(@W64). move => aibnd ai1bnd.
+
+move : bbs; rewrite /signed_bound_cxq => /> bbs. 
+ move : (bbs ( (4*i{hr} + 3)) _); first by smt().
+ move : (bbs (4*i{hr} + 2) _); first by smt(@W64). move => bibnd bi1bnd.
+
+split. split.
+
+move => k kl kh.
+case (k = 4 * i{hr}+2). smt(@Array256 @Fq). 
+case (k = 4 * i{hr}+3). smt(@Array256 @Fq). 
+
+move => *.
+rewrite Array256.set_neqiE; first 2 by smt(@W64). 
+rewrite Array256.set_neqiE; first 2 by smt(@W64). 
+
+move : rb. rewrite /signed_bound_cxq => rb. 
+move : (rb k). rewrite b16E.
+smt(@Fq).
+
+split. 
+
+rewrite /base_mul.
+move => k kb.
+rewrite /lift_array256 !mapiE; first 12 by smt(). 
+
+rewrite !Array256.set_neqiE; first 16 by smt(@W64). 
+
+simplify => />.
+
+move : rv; rewrite /base_mul => rv.
+
+move : (rv k kb).
+rewrite /lift_array256 !mapiE; first 12 by smt(). 
+simplify => />.
+
+move : (SREDCp_corr (to_sint ap{hr}.[4 * i{hr}+2] * to_sint bp{hr}.[4 * i{hr} + 3]) _ _) => />;
+  first 2 by smt(@Fq). 
+
+rewrite eq_inzmod -rval !inzmodM. 
+move => ?? rrval.
+
+
+move : (SREDCp_corr (to_sint ap{hr}.[4 * i{hr} + 3] * to_sint bp{hr}.[4 * i{hr}+2]) _ _) => />;
+  first 2 by smt(@Fq). 
+
+rewrite eq_inzmod -rvall !inzmodM. 
+move => ?? rrvall.
+
+rewrite Array256.set_neqiE; first 2 by smt(@W64). 
+rewrite Array256.set_neqiE; first 2 by smt(@W64). 
+rewrite Array256.set_neqiE; first 2 by smt(@W64). 
+rewrite Array256.set_neqiE; first 2 by smt(@W64). 
+
+split ;  by smt().
+
+
+move : (SREDCp_corr (to_sint ap{hr}.[4 * i{hr}+2] * to_sint bp{hr}.[4 * i{hr} + 3]) _ _) => />;
+  first 2 by smt(@Fq). 
+
+rewrite eq_inzmod -rval !inzmodM. 
+move => ?? rrval.
+
+
+move : (SREDCp_corr (to_sint ap{hr}.[4 * i{hr} + 3] * to_sint bp{hr}.[4 * i{hr}+2]) _ _) => />;
+  first 2 by smt(@Fq). 
+
+rewrite eq_inzmod -rvall !inzmodM. 
+move => ?? rrvall.
+
+rewrite Array256.set_neqiE; first 2 by smt(@W64). 
+rewrite Array256.set_eqiE; first 2 by smt(@W64). 
+rewrite Array256.set_eqiE; first 2 by smt(@W64). 
+
+
+rewrite !to_sintD_small. smt(@Fq).
+rewrite r0val inzmodD rrval rrvall.
+split. split; by ring.
+smt(@W16 @Fq).
+
+(**** FINAL GOAL *)
+ auto => />.
+move => &hr mont bas bbs ?? rb rv ???????? zval zbl zbh  r0val ???rval ?. 
+
+split; first by  smt(@W64).
+split; first by smt().
+split.
+rewrite /signed_bound_cxq => /> k kb.
+case (k < 4*i{hr}).
+   move : rb; rewrite /signed_bound_cxq => /> /#. 
+case (k = 4*i{hr}); smt(@Array256 @Fq).
+
+rewrite /base_mul =>  k kb.
+case (k < i{hr}). 
+   move => *.
+   move : rv; rewrite /base_mul => /> rv.
+   move : (rv k _); rewrite /double_mul /complex_mul => /> /#. 
+move => *. 
+rewrite (_: k = i{hr}); first by smt().
+rewrite /double_mul /complex_mul /lift_array256.
+split. split. 
+rewrite !mapiE; first 6 by smt() => />. 
+rewrite !mapiE; first 6 by smt() => />. 
+rewrite !mapiE; first 6 by smt() => />. 
+smt().
+qed.
+
+end KyberPoly.
