proof/correctness/W16extra.ec
@@ -1,0 +1,80 @@
+require import List Int IntExtra IntDiv CoreMap IntDiv.
+from Jasmin require  import JModel JMemory.
+
+(*
+MOVE ELSEWHERE
+*)
+op b16 (a : W16.t) (b : int) = 
+     -b <= to_sint a < b axiomatized by b16E.
+
+op bpos16 (a : W16.t) (b : int) = 
+     0 <= to_sint a < b  axiomatized by bpos16E.
+
+op bw16 (a : W16.t) i =
+     -2^i <= to_sint a < 2^i  axiomatized by bw16E.
+
+hint simplify b16E.
+hint simplify bpos16E.
+hint simplify bw16E.
+
+lemma to_sintD_small : (forall (a b : W16.t), 
+    -W16.modulus %/2 <= to_sint a + to_sint b < W16.modulus %/2 =>
+    to_sint (a + b) = to_sint a + to_sint b).
+proof. 
+move => a b.
+  rewrite !W16.to_sintE !/smod => />.
+  move : (W16.to_uint_cmp a) (W16.to_uint_cmp b) => /> *.
+  have sumbnd : to_uint a + to_uint b < 65536+65536 ; first  by smt(). 
+  case (65536  <= to_uint a + to_uint b).
++    move => *; rewrite (_:  to_uint (a + b)= (to_uint a +  to_uint b) - 65536);
+       [rewrite to_uintD => />; by  smt(@IntDiv @W16) |  smt(@W16)].
++    move => *; rewrite (_:  to_uint (a + b)= (to_uint a +  to_uint b));
+       [rewrite to_uintD_small => />; by  smt(@IntDiv @W16) |  smt(@W16)].
+qed.
+
+
+lemma to_sintB_small : (forall (a b : W16.t), 
+    -W16.modulus %/2 <= to_sint a - to_sint b < W16.modulus %/2 =>
+    to_sint (a - b) = to_sint a - to_sint b).
+proof.
+  move => a b.
+  rewrite !W16.to_sintE !/smod => />.
+  move : (W16.to_uint_cmp a) (W16.to_uint_cmp b). 
+  case (to_uint b <= to_uint a).
++ case(32768 <= to_uint a); 
+    by move => *;
+      rewrite (_:  to_uint (a - b)= (to_uint a -  to_uint b)); smt(@W16 @IntDiv).
++ case(32768 <= to_uint a);  by 
+    move => /> *; rewrite (_:  to_uint (a - b)= (to_uint a -  to_uint b) + 65536);
+      [rewrite to_uintD to_uintN => />;  smt(@W16 @IntDiv)| smt(@W16 @IntDiv)].
+qed.
+
+lemma to_sintM_small : (forall (a b : W16.t), 
+    -W16.modulus %/2 <= to_sint a * to_sint b < W16.modulus %/2 =>
+    to_sint (a * b) = to_sint a * to_sint b).
+proof.
+move => a b.
+  rewrite !W16.to_sintE !/smod => />.
+  move : (W16.to_uint_cmp a) (W16.to_uint_cmp b) => *.
+  case(32768 <= to_uint a);
+    case(32768 <= to_uint b);
+      by case (65536  <= to_uint a * to_uint b);
+       move => *;rewrite to_uintM  => />;  smt(@W16 @IntDiv). 
+qed.
+
+lemma to_sintN (a : W16.t) : 
+      -W16.modulus %/2 < to_sint a < W16.modulus %/2 =>
+      to_sint (- a) = - to_sint a.
+proof. 
+    rewrite !to_sintE /smod !to_uintN=> /> *. 
+    move : (W16.to_uint_cmp a) => /> *. 
+    case (to_uint a = 0); first by smt(@IntDiv @W16).
+    case (to_uint a = 65535); first by smt(@W16).
+    move => *.
+    rewrite (_: (- to_uint a) %% 65536 = 65536 - to_uint a);
+           smt(@IntDiv @W16 @IntExtra).
+qed.
+
+(*
+END MOVE ELSEWHERE
+*)
